src/go_lang/refinement.v
@@ -1,0 +1,109 @@
+From iris.algebra Require Import auth frac agree gmap list excl.
+From iris.base_logic.lib Require Import invariants.
+From iris.proofmode Require Import tactics.
+From iris.program_logic Require Export language.
+From iris.program_logic Require Import lifting.
+From Perennial.program_logic Require Import refinement.
+From Perennial.go_lang Require Export lang.
+From Perennial.go_lang Require Import tactics notation map lifting.
+
+(* Wrapper around ffi_models and so on to avoid clashes between the ffi for
+   the spec and the concrete *)
+
+Class spec_ffi_model := { spec_ffi_model_field : ffi_model }.
+Class spec_ext_op := { spec_ext_op_field : ext_op }.
+Class spec_ext_semantics (H1: spec_ext_op) (H2: spec_ffi_model) :=
+  { spec_ext_semantics_field : ext_semantics (spec_ext_op_field) (spec_ffi_model_field) }.
+Class spec_ffi_interp (spec_ffi: spec_ffi_model) :=
+  { spec_ffi_interp_field : ffi_interp (spec_ffi_model_field) }.
+
+Section go_refinement.
+Context {spec_ext: spec_ext_op}.
+Context {spec_ffi: spec_ffi_model}.
+Context {spec_ffi_semantics: spec_ext_semantics spec_ext spec_ffi}.
+Context `{!spec_ffi_interp spec_ffi}.
+Canonical Structure spec_lang : language :=
+  @heap_lang (spec_ext_op_field) (spec_ffi_model_field) (spec_ext_semantics_field).
+
+Existing Instance spec_ffi_interp_field.
+Existing Instance spec_ext_semantics_field.
+Existing Instance spec_ext_op_field.
+Existing Instance spec_ffi_model_field.
+
+
+Class refinement_heapG Σ := refinement_HeapG {
+  refinement_spec_ffiG : ffiG Σ;
+  refinement_traceG :> traceG Σ;
+  refinement_cfgG :> @cfgG spec_lang Σ;
+  refinement_gen_heapG :> gen_heapG loc (nonAtomic (@val spec_ext_op_field)) Σ;
+  (* TODO: do we need prophecies at the spec level? *)
+  (*
+  refinement_proph_mapG :> proph_mapG proph_id (val * val) Σ;
+   *)
+}.
+
+Context {Σ: gFunctors}.
+Context {hR: refinement_heapG Σ}.
+Context `{invG Σ}.
+
+Definition spec_interp σ : iProp Σ :=
+    (gen_heap_ctx σ.(heap) ∗ (* proph_map_ctx κs σ.(used_proph_id) ∗ *) ffi_ctx refinement_spec_ffiG σ.(world)
+      ∗ trace_auth σ.(trace))%I.
+
+Definition spec_stateN := nroot .@ "source".@  "state".
+
+(* TODO: these names are terrible *)
+Definition spec_ctx : iProp Σ :=
+  source_ctx ∗ inv spec_stateN (∃ σ, source_state σ ∗ spec_interp σ)%I.
+
+Global Instance spec_ctx_persistent : Persistent (spec_ctx).
+Proof. apply _. Qed.
+
+(** Override the notations so that scopes and coercions work out *)
+Notation "l s↦{ q } v" := (mapsto (L:=loc) (V:=nonAtomic val) (hG := refinement_heapG) l q v%V)
+  (at level 20, q at level 50, format "l  s↦{ q }  v") : bi_scope.
+Notation "l s↦ v" :=
+  (mapsto (L:=loc) (V:=nonAtomic val) (hG := refinement_heapG) l 1 v%V) (at level 20) : bi_scope.
+Notation "l s↦{ q } -" := (∃ v, l ↦{q} v)%I
+  (at level 20, q at level 50, format "l  s↦{ q }  -") : bi_scope.
+Notation "l ↦ -" := (l ↦{1} -)%I (at level 20) : bi_scope.
+
+Section go_ghost_step.
+
+Lemma sourceN_sub_minus_state E:
+  nclose sourceN_root ⊆ E →
+  nclose sourceN ⊆ E ∖ ↑spec_stateN.
+Proof.
+  rewrite /sourceN/sourceN_root/spec_stateN. intros Hsub.
+  assert (nclose (nroot.@"source".@"base") ##
+                 ↑nroot.@"source".@"state").
+  { solve_ndisj. }
+  assert (nclose (nroot.@"source".@"base") ⊆ E).
+  { etransitivity; last eassumption. apply nclose_subseteq. }
+  set_solver.
+Qed.
+
+Hint Resolve sourceN_sub_minus_state.
+
+Lemma ghost_load j K E l q v:
+  nclose sourceN_root ⊆ E →
+  spec_ctx -∗
+  l ↦{q} Free v -∗
+  j ⤇ fill K (Load (Val $ LitV $ LitLoc l)) ={E}=∗
+  l ↦{q} Free v ∗ j ⤇ fill K v.
+Proof.
+  iIntros (?) "(#Hctx&#Hstate) Hl Hj".
+  iInv "Hstate" as (?) "(>H&Hinterp)" "Hclo".
+  iDestruct "Hinterp" as "(>Hσ&Hrest)".
+  iDestruct (@gen_heap_valid with "Hσ Hl") as %?.
+  iMod (ghost_step_lifting with "Hj Hctx H") as "(Hj&H&_)".
+  { eapply head_prim_step; econstructor; eauto. }
+  { eauto. }
+  iMod ("Hclo" with "[Hσ H Hrest]").
+  { iNext. iExists _. iFrame. }
+  iFrame. eauto.
+Qed.
+
+End go_ghost_step.
+
+End go_refinement.
